WIP: proving new and better lib typing

translation/Library.v
@@ -3,6 +3,7 @@ This file shows typing of the `lib` term encoding the primitives of the source c
 *)
 Require Import Helpers.
 
+Parameter Any : typ_label.
 Parameter Unit : typ_label.
 Parameter Tuple : typ_label.
 Parameter GenT : typ_label.
@@ -22,7 +23,9 @@ Parameter pmatch : trm_label.
 Axiom diff : Unit <> Tuple
              /\ mkUnit <> mkTuple
              /\ T1 <> T2
-             /\ fst_v <> snd_v.
+             /\ fst_v <> snd_v
+             /\ Any <> Tuple
+             /\ Any <> Unit.
 
 (* Generating some fresh vars *)
 Definition lib : var := proj1_sig (var_fresh \{}).
@@ -53,6 +56,7 @@ Definition GenArgT : Target.typ :=
   typ_rcd { GenT >: ⊥ <: ⊤ }.
 
 Definition libPreTypeHelp (unitDec : dec) : typ :=
+  typ_rcd { Any == ⊤ } ∧
   typ_rcd unitDec ∧
   typ_rcd { Tuple == tupleTyp } ∧
   typ_rcd { mkUnit ⦂ this ↓ Unit } ∧
@@ -64,7 +68,7 @@ Definition libPreTypeHelp (unitDec : dec) : typ :=
           }.
 
 Definition libPreType : Target.typ :=
-  libPreTypeHelp { Unit == { Unit >: ⊥ <: ⊤ } }.
+  libPreTypeHelp { Unit == { Unit >: ⊥ <: ⊤ } } .
 
 Definition libType : Target.typ :=
   μ (libPreTypeHelp { Unit >: ⊥ <: ⊤ }).
@@ -76,9 +80,10 @@ Definition internalTupleTyp :=
   { snd_v ⦂ {{ ref 1 }} }.
 
 Definition libInternalType (unitRef : path) :=
+  typ_rcd { Any == ⊤ } ∧
   typ_rcd { Unit == { Unit >: ⊥ <: ⊤ } } ∧
   typ_rcd { Tuple == tupleTyp } ∧
-  typ_rcd { mkUnit ⦂ {{ unitRef }} } ∧
+  typ_rcd { mkUnit ⦂ μ({Unit == ⊤}) } ∧
   typ_rcd { mkTuple ⦂
                     ∀ ({ T1 >: ⊥ <: ⊤} ∧ { T2 >: ⊥ <: ⊤ })
                         ∀ ((ref 0) ↓ T1)
@@ -86,277 +91,312 @@ Definition libInternalType (unitRef : path) :=
                               ((ref 3) ↓ Tuple ∧ { T1 == (ref 2) ↓ T1 } ∧ { T2 == (ref 2) ↓ T2 })
           }.
 
-(* Definition libTrm : Target.trm := *)
-(*   trm_let *)
-(*     (let_trm (ν({ Unit == ⊤ }) {( {Unit ⦂= ⊤} )})) *)
-(*   (let_trm *)
-(*     (ν(libInternalType (ref 1)) {( *)
-(*                            { Unit ⦂= { Unit >: ⊥ <: ⊤ } }, *)
-(*                            { Tuple ⦂= tupleTyp }, *)
-(*                            { mkUnit := ref 1 }, *)
-(*                            { mkTuple := *)
-(*                                λ ({ T1 >: ⊥ <: ⊤} ∧ { T2 >: ⊥ <: ⊤ }) *)
-(*                                  λ ((ref 0) ↓ T1) *)
-(*                                  λ ((ref 1) ↓ T2) *)
-(*                                  let_trm ( *)
-(*                                    ν(internalTupleTyp) *)
-(*                                     {( *)
-(*                                         {T1 ⦂= (ref 3) ↓ T1}, *)
-(*                                         {T2 ⦂= (ref 3) ↓ T2}, *)
-(*                                         { fst_v := (ref 2) }, *)
-(*                                         { snd_v := (ref 1) } *)
-(*                                     )} *)
-(*                                  ) *)
-(*                            } *)
-(*                         )} *)
-(*     )) *)
-(*  . *)
+Definition libTrm : Target.trm :=
+  (let_trm
+    (ν[ref 0 ↘ Any](libInternalType (ref 1)) {(
+                           { Unit ⦂= { Unit >: ⊥ <: ⊤ } },
+                           { Tuple ⦂= tupleTyp },
+                           { mkUnit := ν[ref 0 ↘ Unit]({ Unit == ⊤ }) {( {Unit ⦂= ⊤} )} },
+                           { mkTuple :=
+                               λ ({ T1 >: ⊥ <: ⊤} ∧ { T2 >: ⊥ <: ⊤ })
+                                 λ ((ref 0) ↓ T1)
+                                 λ ((ref 1) ↓ T2)
+                                 let_trm (
+                                   ν[ref 3 ↘ Tuple](internalTupleTyp)
+                                    {(
+                                        {T1 ⦂= (ref 3) ↓ T1},
+                                        {T2 ⦂= (ref 3) ↓ T2},
+                                        { fst_v := (ref 2) },
+                                        { snd_v := (ref 1) }
+                                    )}
+                                 )
+                           }
+                        )}
+    ))
+ .
 
-(* Lemma libTypes : forall G, G ⊢ libTrm : libType. *)
-(* Proof. *)
-(*   intros. *)
-(*   unfold libTrm. unfold libType. *)
-(*   let F := gather_vars in *)
-(*   apply ty_let with F ({ Unit >: ⊥ <: ⊤ }). *)
-(*   1: { *)
-(*     let F := gather_vars in *)
-(*     apply ty_let with F (μ { Unit == ⊤ }). *)
-(*     - apply_fresh ty_new_intro as u. *)
-(*       crush. *)
-(*     - intros u Fru. *)
-(*       crush. *)
-(*       apply ty_sub with {Unit == ⊤}. *)
-(*       + assert (HU: typ_rcd {Unit == ⊤} = open_typ_p (pvar u) {Unit == ⊤}) by crush. *)
-(*         rewrite HU. *)
-(*         apply ty_rec_elim. *)
-(*         apply~ ty_var. *)
-(*       + apply~ subtyp_typ. *)
-(*   } *)
+Lemma libTypes : forall G, G ⊢ libTrm : libType.
+Proof.
+  intros.
+  unfold libTrm. unfold libType.
+  let F := gather_vars in
+  apply ty_let with F (μ libInternalType this).
+  2: {
+    unfold libInternalType.
+    unfold libPreTypeHelp.
+    cbn. case_if.
+    introv F.
+    apply ty_rec_intro.
+    cbn. repeat case_if.
+    unfold tupleTyp.
+    repeat (apply ty_and_intro; try solve [var_subtyp_mu2; solve_subtyp_and]).
+    - var_subtyp_mu2.
+      apply subtyp_trans with ({Unit == {Unit >: ⊥ <: ⊤} });
+        solve_subtyp_and; auto.
+    - apply ty_rcd_intro.
+      apply ty_sub with {Unit == ⊤}.
+      + cbn.
+        assert (HR: typ_rcd {Unit == ⊤} = open_typ_p (p_sel (avar_f x) [mkUnit]) {Unit == ⊤}) by crush;
+          rewrite HR; clear HR.
+        apply ty_rec_elim.
+        assert (HR: (trm_path (pvar x) • mkUnit) = trm_path (p_sel (avar_f x) [mkUnit])) by crush;
+          rewrite <- HR; clear HR.
+        apply ty_new_elim.
+        var_subtyp_mu2. solve_subtyp_and.
+      + eapply subtyp_sel2.
+        var_subtyp_mu2.
+        eapply subtyp_trans; try apply subtyp_and11.
+        eapply subtyp_trans; try apply subtyp_and11.
+        eapply subtyp_trans; try apply subtyp_and11.
+        eapply subtyp_trans; try apply subtyp_and12.
+        apply~ subtyp_typ.
+  }
 
-(*   intros u Fru. *)
-(*   crush. *)
-(*   let F := gather_vars in *)
-(*   apply ty_let with F (μ libInternalType (pvar u)). *)
-(*   - cbv. *)
-(*     apply_fresh ty_new_intro as z. *)
-(*     crush. *)
-(*     repeat apply ty_defs_cons; try apply ty_defs_one. *)
-(*     + apply ty_def_typ. *)
-(*     + apply ty_def_typ. *)
-(*     + crush. destructs diff. false. *)
-(*     + apply~ ty_def_path. *)
-(*     + crush. *)
-(*     + apply ty_def_all. *)
-(*       apply_fresh ty_all_intro as tl. *)
-(*       apply_fresh ty_all_intro as x1. *)
-(*       apply_fresh ty_all_intro as x2. *)
-(*       cbv. repeat case_if. *)
-(*       clear - Frz Frtl Frx1 Frx2. *)
-(*       eapply ty_let. *)
-(*       * apply_fresh ty_new_intro as w. *)
-(*         crush. *)
-(*         repeat apply ty_defs_cons; try apply ty_defs_one; *)
-(*           auto; try crush. *)
-(*         -- inversion C. destructs diff. false. *)
-(*         -- apply~ ty_def_path. *)
-(*         -- apply~ ty_def_path. *)
-(*         -- inversion C. destructs diff. false. *)
-(*       * crush. *)
-(*         let F := gather_vars in *)
-(*         intros tup Frtup; *)
-(*           instantiate (1:=F) in Frtup. *)
-(*         repeat apply ty_and_intro. *)
-(*         -- eapply ty_sub with (μ (({T1 >: ⊥ <: ⊤} ∧ {T2 >: ⊥ <: ⊤}) ∧ {fst_v ⦂ this ↓ T1}) ∧ {snd_v ⦂ this ↓ T2}). *)
-(*            ++ apply ty_rec_intro. *)
-(*               crush. *)
-(*               repeat apply ty_and_intro. *)
-(*               ** match goal with *)
-(*                  | [ |- context[tup ~ μ ?T] ] => *)
-(*                    apply ty_sub with T *)
-(*                  end. *)
-(*                  --- match goal with *)
-(*                      | [ |- ?G ⊢ tvar tup : ?T ] => *)
-(*                        assert (Hre: T = open_typ_p (pvar tup) T) by (cbn; auto); *)
-(*                          rewrite Hre; *)
-(*                          clear Hre *)
-(*                      end. *)
-(*                      apply ty_rec_elim. cbn. apply~ ty_var. *)
-(*                  --- eapply subtyp_trans; try apply subtyp_and11. *)
-(*                      eapply subtyp_trans; try apply subtyp_and11. *)
-(*                      eapply subtyp_trans; try apply subtyp_and11. *)
-(*                      apply~ subtyp_typ. *)
-(*               ** match goal with *)
-(*                  | [ |- context[tup ~ μ ?T] ] => *)
-(*                    apply ty_sub with T *)
-(*                  end. *)
-(*                  --- match goal with *)
-(*                      | [ |- ?G ⊢ tvar tup : ?T ] => *)
-(*                        assert (Hre: T = open_typ_p (pvar tup) T) by (cbn; auto); *)
-(*                          rewrite Hre; *)
-(*                          clear Hre *)
-(*                      end. *)
-(*                      apply ty_rec_elim. cbn. apply~ ty_var. *)
-(*                  --- eapply subtyp_trans; try apply subtyp_and11. *)
-(*                      eapply subtyp_trans; try apply subtyp_and11. *)
-(*                      eapply subtyp_trans; try apply subtyp_and12. *)
-(*                      apply~ subtyp_typ. *)
-(*               ** apply ty_rcd_intro. *)
-(*                  apply ty_sngl with (pvar x1). *)
-(*                  --- apply ty_new_elim. *)
-(*                      match goal with *)
-(*                      | [ |- context[tup ~ μ ?T] ] => *)
-(*                        apply ty_sub with T *)
-(*                      end. *)
-(*                      +++ match goal with *)
-(*                          | [ |- ?G ⊢ tvar tup : ?T ] => *)
-(*                            assert (Hre: T = open_typ_p (pvar tup) T) by (cbn; auto); *)
-(*                              rewrite Hre; *)
-(*                              clear Hre *)
-(*                          end. *)
-(*                          apply ty_rec_elim. cbn. apply~ ty_var. *)
-(*                      +++ eapply subtyp_trans; try apply subtyp_and11. *)
-(*                          eapply subtyp_trans; try apply subtyp_and12. *)
-(*                          apply subtyp_refl. *)
-(*                  --- apply ty_sub with (pvar tl ↓ T1). *)
-(*                      +++ auto. *)
-(*                      +++ eapply subtyp_sel2. *)
-(*                          match goal with *)
-(*                          | [ |- context[tup ~ μ ?T] ] => *)
-(*                            apply ty_sub with T *)
-(*                          end. *)
-(*                          *** match goal with *)
-(*                              | [ |- ?G ⊢ tvar tup : ?T ] => *)
-(*                                assert (Hre: T = open_typ_p (pvar tup) T) by (cbn; auto); *)
-(*                                  rewrite Hre; *)
-(*                                  clear Hre *)
-(*                              end. *)
-(*                              apply ty_rec_elim. cbn. apply~ ty_var. *)
-(*                          *** eapply subtyp_trans; try apply subtyp_and11. *)
-(*                              eapply subtyp_trans; try apply subtyp_and11. *)
-(*               ** apply ty_rcd_intro. *)
-(*                  apply ty_sngl with (pvar x2). *)
-(*                  --- apply ty_new_elim. *)
-(*                      match goal with *)
-(*                      | [ |- context[tup ~ μ ?T] ] => *)
-(*                        apply ty_sub with T *)
-(*                      end. *)
-(*                      +++ match goal with *)
-(*                          | [ |- ?G ⊢ tvar tup : ?T ] => *)
-(*                            assert (Hre: T = open_typ_p (pvar tup) T) by (cbn; auto); *)
-(*                              rewrite Hre; *)
-(*                              clear Hre *)
-(*                          end. *)
-(*                          apply ty_rec_elim. cbn. apply~ ty_var. *)
-(*                      +++ eapply subtyp_trans; try apply subtyp_and12. *)
-(*                          apply subtyp_refl. *)
-(*                  --- apply ty_sub with (pvar tl ↓ T2). *)
-(*                      +++ auto. *)
-(*                      +++ eapply subtyp_sel2. *)
-(*                          match goal with *)
-(*                          | [ |- context[tup ~ μ ?T] ] => *)
-(*                            apply ty_sub with T *)
-(*                          end. *)
-(*                          *** match goal with *)
-(*                              | [ |- ?G ⊢ tvar tup : ?T ] => *)
-(*                                assert (Hre: T = open_typ_p (pvar tup) T) by (cbn; auto); *)
-(*                                  rewrite Hre; *)
-(*                                  clear Hre *)
-(*                              end. *)
-(*                              apply ty_rec_elim. cbn. apply~ ty_var. *)
-(*                          *** eapply subtyp_trans; try apply subtyp_and11. *)
-(*                              eapply subtyp_trans; try apply subtyp_and11. *)
-(*                              eapply subtyp_trans; try apply subtyp_and12. *)
-(*                              auto. *)
-(*            ++ eapply subtyp_sel2. *)
-(*               match goal with *)
-(*               | [ |- context [z ~ ?T] ] => *)
-(*                 apply ty_sub with T *)
-(*               end. *)
-(*               ** apply~ ty_var. *)
-(*               ** eapply subtyp_trans; try apply subtyp_and11. *)
-(*                  eapply subtyp_trans; try apply subtyp_and11. *)
-(*                  apply subtyp_and12. *)
-(*         -- apply ty_sub with (({T1 == pvar tl ↓ T1} ∧ {T2 == pvar tl ↓ T2}) ∧ {fst_v ⦂ {{pvar x1}}} ∧ {snd_v ⦂ {{pvar x2}}}). *)
-(*            ++ match goal with *)
-(*               | [ |- ?G ⊢ tvar tup : ?T ] => *)
-(*                 assert (Hre: T = open_typ_p (pvar tup) T) by (cbn; auto); *)
-(*                   rewrite Hre; *)
-(*                   clear Hre *)
-(*               end. *)
-(*               apply ty_rec_elim. *)
-(*               cbn in *. *)
-(*               apply ty_var. auto. *)
-(*            ++ repeat (eapply subtyp_trans; try apply subtyp_and11). *)
-(*         -- apply ty_sub with (({T1 == pvar tl ↓ T1} ∧ {T2 == pvar tl ↓ T2}) ∧ {fst_v ⦂ {{pvar x1}}} ∧ {snd_v ⦂ {{pvar x2}}}). *)
-(*            ++ match goal with *)
-(*               | [ |- ?G ⊢ tvar tup : ?T ] => *)
-(*                 assert (Hre: T = open_typ_p (pvar tup) T) by (cbn; auto); *)
-(*                   rewrite Hre; *)
-(*                   clear Hre *)
-(*               end. *)
-(*               apply ty_rec_elim. *)
-(*               cbn in *. *)
-(*               apply ty_var. auto. *)
-(*            ++ eapply subtyp_trans; try apply subtyp_and11. *)
-(*               eapply subtyp_trans; try apply subtyp_and11. *)
-(*               apply subtyp_and12. *)
-(*     + crush. *)
-(*       inversion C17. destructs diff. false. *)
-(*   - intros x Frx. *)
-(*     cbv. crush. *)
-(*     apply ty_rec_intro. *)
-(*     crush. *)
-(*     repeat apply ty_and_intro. *)
-(*     + match goal with *)
-(*       | [ |- context [ x ~ (μ ?B) ] ] => *)
-(*         apply ty_sub with (open_typ_p (pvar x) B) *)
-(*       end. *)
-(*       * apply~ ty_rec_elim. *)
-(*       * crush. *)
-(*         eapply subtyp_trans; try apply subtyp_and11. *)
-(*         eapply subtyp_trans; try apply subtyp_and11. *)
-(*         eapply subtyp_trans; try apply subtyp_and11. *)
-(*         apply~ subtyp_typ. *)
-(*     + match goal with *)
-(*       | [ |- context [ x ~ (μ ?B) ] ] => *)
-(*         apply ty_sub with (open_typ_p (pvar x) B) *)
-(*       end. *)
-(*       * apply~ ty_rec_elim. *)
-(*       * crush. *)
-(*         eapply subtyp_trans; try apply subtyp_and11. *)
-(*         eapply subtyp_trans; try apply subtyp_and11. *)
-(*         eapply subtyp_trans; try apply subtyp_and12. *)
-(*         apply~ subtyp_refl. *)
-(*     + apply ty_rcd_intro. *)
-(*       apply ty_sngl with (pvar u). *)
-(*       * apply ty_new_elim. *)
-(*         match goal with *)
-(*         | [ |- context [ x ~ (μ ?B) ] ] => *)
-(*           apply ty_sub with (open_typ_p (pvar x) B) *)
-(*         end. *)
-(*         -- apply~ ty_rec_elim. *)
-(*         -- crush. *)
-(*            eapply subtyp_trans; try apply subtyp_and11. *)
-(*            eapply subtyp_trans; try apply subtyp_and12. *)
-(*            apply subtyp_refl. *)
-(*       * apply ty_sub with ({Unit >: ⊥ <: ⊤}). *)
-(*         -- auto. *)
-(*         -- eapply subtyp_sel2. *)
-(*            match goal with *)
-(*            | [ |- context [ x ~ (μ ?B) ] ] => *)
-(*              apply ty_sub with (open_typ_p (pvar x) B) *)
-(*            end. *)
-(*            ++ apply~ ty_rec_elim. *)
-(*            ++ crush. *)
-(*               eapply subtyp_trans; try apply subtyp_and11. *)
-(*               eapply subtyp_trans; try apply subtyp_and11. *)
-(*     + match goal with *)
-(*       | [ |- context [ x ~ (μ ?B) ] ] => *)
-(*         apply ty_sub with (open_typ_p (pvar x) B) *)
-(*       end. *)
-(*       ++ apply~ ty_rec_elim. *)
-(*       ++ crush. *)
-(* Qed. *)
+  unfold libInternalType.
+  cbn.
+
+  unfold libPreTypeHelp.
+  unfold libInternalType.
+  apply ty_new_intro.
+  1: {
+    let F := gather_vars in
+    apply ty_let with F (μ { Unit == ⊤ }).
+    - apply_fresh ty_new_intro as u.
+      crush.
+    - intros u Fru.
+      crush.
+      apply ty_sub with {Unit == ⊤}.
+      + assert (HU: typ_rcd {Unit == ⊤} = open_typ_p (pvar u) {Unit == ⊤}) by crush.
+        rewrite HU.
+        apply ty_rec_elim.
+        apply~ ty_var.
+      + apply~ subtyp_typ.
+  }
+
+  intros u Fru.
+  crush.
+  let F := gather_vars in
+  apply ty_let with F (μ libInternalType (pvar u)).
+  - cbv.
+    apply_fresh ty_new_intro as z.
+    crush.
+    repeat apply ty_defs_cons; try apply ty_defs_one.
+    + apply ty_def_typ.
+    + apply ty_def_typ.
+    + crush. destructs diff. false.
+    + apply~ ty_def_path.
+    + crush.
+    + apply ty_def_all.
+      apply_fresh ty_all_intro as tl.
+      apply_fresh ty_all_intro as x1.
+      apply_fresh ty_all_intro as x2.
+      cbv. repeat case_if.
+      clear - Frz Frtl Frx1 Frx2.
+      eapply ty_let.
+      * apply_fresh ty_new_intro as w.
+        crush.
+        repeat apply ty_defs_cons; try apply ty_defs_one;
+          auto; try crush.
+        -- inversion C. destructs diff. false.
+        -- apply~ ty_def_path.
+        -- apply~ ty_def_path.
+        -- inversion C. destructs diff. false.
+      * crush.
+        let F := gather_vars in
+        intros tup Frtup;
+          instantiate (1:=F) in Frtup.
+        repeat apply ty_and_intro.
+        -- eapply ty_sub with (μ (({T1 >: ⊥ <: ⊤} ∧ {T2 >: ⊥ <: ⊤}) ∧ {fst_v ⦂ this ↓ T1}) ∧ {snd_v ⦂ this ↓ T2}).
+           ++ apply ty_rec_intro.
+              crush.
+              repeat apply ty_and_intro.
+              ** match goal with
+                 | [ |- context[tup ~ μ ?T] ] =>
+                   apply ty_sub with T
+                 end.
+                 --- match goal with
+                     | [ |- ?G ⊢ tvar tup : ?T ] =>
+                       assert (Hre: T = open_typ_p (pvar tup) T) by (cbn; auto);
+                         rewrite Hre;
+                         clear Hre
+                     end.
+                     apply ty_rec_elim. cbn. apply~ ty_var.
+                 --- eapply subtyp_trans; try apply subtyp_and11.
+                     eapply subtyp_trans; try apply subtyp_and11.
+                     eapply subtyp_trans; try apply subtyp_and11.
+                     apply~ subtyp_typ.
+              ** match goal with
+                 | [ |- context[tup ~ μ ?T] ] =>
+                   apply ty_sub with T
+                 end.
+                 --- match goal with
+                     | [ |- ?G ⊢ tvar tup : ?T ] =>
+                       assert (Hre: T = open_typ_p (pvar tup) T) by (cbn; auto);
+                         rewrite Hre;
+                         clear Hre
+                     end.
+                     apply ty_rec_elim. cbn. apply~ ty_var.
+                 --- eapply subtyp_trans; try apply subtyp_and11.
+                     eapply subtyp_trans; try apply subtyp_and11.
+                     eapply subtyp_trans; try apply subtyp_and12.
+                     apply~ subtyp_typ.
+              ** apply ty_rcd_intro.
+                 apply ty_sngl with (pvar x1).
+                 --- apply ty_new_elim.
+                     match goal with
+                     | [ |- context[tup ~ μ ?T] ] =>
+                       apply ty_sub with T
+                     end.
+                     +++ match goal with
+                         | [ |- ?G ⊢ tvar tup : ?T ] =>
+                           assert (Hre: T = open_typ_p (pvar tup) T) by (cbn; auto);
+                             rewrite Hre;
+                             clear Hre
+                         end.
+                         apply ty_rec_elim. cbn. apply~ ty_var.
+                     +++ eapply subtyp_trans; try apply subtyp_and11.
+                         eapply subtyp_trans; try apply subtyp_and12.
+                         apply subtyp_refl.
+                 --- apply ty_sub with (pvar tl ↓ T1).
+                     +++ auto.
+                     +++ eapply subtyp_sel2.
+                         match goal with
+                         | [ |- context[tup ~ μ ?T] ] =>
+                           apply ty_sub with T
+                         end.
+                         *** match goal with
+                             | [ |- ?G ⊢ tvar tup : ?T ] =>
+                               assert (Hre: T = open_typ_p (pvar tup) T) by (cbn; auto);
+                                 rewrite Hre;
+                                 clear Hre
+                             end.
+                             apply ty_rec_elim. cbn. apply~ ty_var.
+                         *** eapply subtyp_trans; try apply subtyp_and11.
+                             eapply subtyp_trans; try apply subtyp_and11.
+              ** apply ty_rcd_intro.
+                 apply ty_sngl with (pvar x2).
+                 --- apply ty_new_elim.
+                     match goal with
+                     | [ |- context[tup ~ μ ?T] ] =>
+                       apply ty_sub with T
+                     end.
+                     +++ match goal with
+                         | [ |- ?G ⊢ tvar tup : ?T ] =>
+                           assert (Hre: T = open_typ_p (pvar tup) T) by (cbn; auto);
+                             rewrite Hre;
+                             clear Hre
+                         end.
+                         apply ty_rec_elim. cbn. apply~ ty_var.
+                     +++ eapply subtyp_trans; try apply subtyp_and12.
+                         apply subtyp_refl.
+                 --- apply ty_sub with (pvar tl ↓ T2).
+                     +++ auto.
+                     +++ eapply subtyp_sel2.
+                         match goal with
+                         | [ |- context[tup ~ μ ?T] ] =>
+                           apply ty_sub with T
+                         end.
+                         *** match goal with
+                             | [ |- ?G ⊢ tvar tup : ?T ] =>
+                               assert (Hre: T = open_typ_p (pvar tup) T) by (cbn; auto);
+                                 rewrite Hre;
+                                 clear Hre
+                             end.
+                             apply ty_rec_elim. cbn. apply~ ty_var.
+                         *** eapply subtyp_trans; try apply subtyp_and11.
+                             eapply subtyp_trans; try apply subtyp_and11.
+                             eapply subtyp_trans; try apply subtyp_and12.
+                             auto.
+           ++ eapply subtyp_sel2.
+              match goal with
+              | [ |- context [z ~ ?T] ] =>
+                apply ty_sub with T
+              end.
+              ** apply~ ty_var.
+              ** eapply subtyp_trans; try apply subtyp_and11.
+                 eapply subtyp_trans; try apply subtyp_and11.
+                 apply subtyp_and12.
+        -- apply ty_sub with (({T1 == pvar tl ↓ T1} ∧ {T2 == pvar tl ↓ T2}) ∧ {fst_v ⦂ {{pvar x1}}} ∧ {snd_v ⦂ {{pvar x2}}}).
+           ++ match goal with
+              | [ |- ?G ⊢ tvar tup : ?T ] =>
+                assert (Hre: T = open_typ_p (pvar tup) T) by (cbn; auto);
+                  rewrite Hre;
+                  clear Hre
+              end.
+              apply ty_rec_elim.
+              cbn in *.
+              apply ty_var. auto.
+           ++ repeat (eapply subtyp_trans; try apply subtyp_and11).
+        -- apply ty_sub with (({T1 == pvar tl ↓ T1} ∧ {T2 == pvar tl ↓ T2}) ∧ {fst_v ⦂ {{pvar x1}}} ∧ {snd_v ⦂ {{pvar x2}}}).
+           ++ match goal with
+              | [ |- ?G ⊢ tvar tup : ?T ] =>
+                assert (Hre: T = open_typ_p (pvar tup) T) by (cbn; auto);
+                  rewrite Hre;
+                  clear Hre
+              end.
+              apply ty_rec_elim.
+              cbn in *.
+              apply ty_var. auto.
+           ++ eapply subtyp_trans; try apply subtyp_and11.
+              eapply subtyp_trans; try apply subtyp_and11.
+              apply subtyp_and12.
+    + crush.
+      inversion C17. destructs diff. false.
+  - intros x Frx.
+    cbv. crush.
+    apply ty_rec_intro.
+    crush.
+    repeat apply ty_and_intro.
+    + match goal with
+      | [ |- context [ x ~ (μ ?B) ] ] =>
+        apply ty_sub with (open_typ_p (pvar x) B)
+      end.
+      * apply~ ty_rec_elim.
+      * crush.
+        eapply subtyp_trans; try apply subtyp_and11.
+        eapply subtyp_trans; try apply subtyp_and11.
+        eapply subtyp_trans; try apply subtyp_and11.
+        apply~ subtyp_typ.
+    + match goal with
+      | [ |- context [ x ~ (μ ?B) ] ] =>
+        apply ty_sub with (open_typ_p (pvar x) B)
+      end.
+      * apply~ ty_rec_elim.
+      * crush.
+        eapply subtyp_trans; try apply subtyp_and11.
+        eapply subtyp_trans; try apply subtyp_and11.
+        eapply subtyp_trans; try apply subtyp_and12.
+        apply~ subtyp_refl.
+    + apply ty_rcd_intro.
+      apply ty_sngl with (pvar u).
+      * apply ty_new_elim.
+        match goal with
+        | [ |- context [ x ~ (μ ?B) ] ] =>
+          apply ty_sub with (open_typ_p (pvar x) B)
+        end.
+        -- apply~ ty_rec_elim.
+        -- crush.
+           eapply subtyp_trans; try apply subtyp_and11.
+           eapply subtyp_trans; try apply subtyp_and12.
+           apply subtyp_refl.
+      * apply ty_sub with ({Unit >: ⊥ <: ⊤}).
+        -- auto.
+        -- eapply subtyp_sel2.
+           match goal with
+           | [ |- context [ x ~ (μ ?B) ] ] =>
+             apply ty_sub with (open_typ_p (pvar x) B)
+           end.
+           ++ apply~ ty_rec_elim.
+           ++ crush.
+              eapply subtyp_trans; try apply subtyp_and11.
+              eapply subtyp_trans; try apply subtyp_and11.
+    + match goal with
+      | [ |- context [ x ~ (μ ?B) ] ] =>
+        apply ty_sub with (open_typ_p (pvar x) B)
+      end.
+      ++ apply~ ty_rec_elim.
+      ++ crush.
+Qed.
 
 Definition TupleT (TT1 TT2 : Target.typ) : Target.typ :=
   (pvar lib ↓ Tuple) ∧ { T1 == TT1 } ∧ { T2 == TT2 }.
